<?xml version="1.0" encoding="UTF-8"?>
<rdf:RDF
	xmlns:skos="http://www.w3.org/2004/02/skos/core#"
	xmlns:cc="http://web.resource.org/cc/"
	xmlns:dctype="http://purl.org/dc/dcmitype/"
	xmlns:dct="http://purl.org/dc/terms/"
	xmlns:vann="http://purl.org/vocab/vann/"
	xmlns:dc="http://purl.org/dc/elements/1.1/"
	xmlns:rdf="http://www.w3.org/1999/02/22-rdf-syntax-ns#"
	xmlns:rdfs="http://www.w3.org/2000/01/rdf-schema#"
	xmlns:owl="http://www.w3.org/2002/07/owl#"
	xmlns:xsd="http://www.w3.org/2001/XMLSchema#">
	<owl:Ontology rdf:about="" dc:date="2008-06-03">
		<dc:title xml:lang="en">Lifecycle Schema</dc:title>
		<rdfs:comment xml:lang="en">
			The Lifecycle Schema provides classes and properties that allow the specification of a lifecycle that any resource may pass through. It's intention to allow the description of the states and transitions that constitute a given lifecycle without imposing any constraint on the way in which transitions happen or how long it may take to move through a lifecycle.
    	</rdfs:comment>
		<dc:identifier>http://purl.org/vocab/lifecycle/schema-20080603</dc:identifier>
		<dct:isVersionOf rdf:resource="http://purl.org/vocab/lifecycle/schema#"/>
		<dc:creator>Rob Styles</dc:creator>
		<dc:creator>Nadeem Shabir</dc:creator>
		<dc:rights>Copyright Â© 2008 Talis Information Ltd</dc:rights>
		<vann:preferredNamespaceUri>http://purl.org/vocab/lifecycle/schema#</vann:preferredNamespaceUri>
		<vann:preferredNamespacePrefix>lifecycle</vann:preferredNamespacePrefix>
		<vann:example rdf:resource="schema-diagram.html" />
		<vann:example rdf:resource="example-job-application-lifecycle.html" />
		<dct:replaces rdf:resource="http://purl.org/vocab/lifecycle/schema-20080603"/>
		<dct:hasFormat>
			<dctype:Text rdf:about="http://purl.org/vocab/lifecycle/schema-20080603.html">
				<dc:format>
					<dct:IMT>
						<rdf:value>text/html</rdf:value>
						<rdfs:label xml:lang="en">HTML</rdfs:label>
					</dct:IMT>
				</dc:format>
			</dctype:Text>
		</dct:hasFormat>
		<dct:hasFormat>
			<dctype:Text rdf:about="http://purl.org/vocab/lifecycle/schema-20080603.rdf">
				<dc:format>
					<dct:IMT>
						<rdf:value>application/rdf+xml</rdf:value>
						<rdfs:label xml:lang="en">RDF</rdfs:label>
					</dct:IMT>
				</dc:format>
			</dctype:Text>
		</dct:hasFormat>
		<dct:issued>2008-06-03</dct:issued>
		<skos:historyNote rdf:value="First cut of the ontology published" dc:date="2008-06-03" dc:creator="Rob Styles"/>
	</owl:Ontology>
	<cc:Work rdf:about="">
		<cc:license rdf:resource="http://creativecommons.org/licenses/by/2.0/uk/"/>
	</cc:Work>
	<cc:License rdf:about="http://creativecommons.org/licenses/by/2.0/uk/">
		<cc:permits rdf:resource="http://web.resource.org/cc/Reproduction"/>
		<cc:permits rdf:resource="http://web.resource.org/cc/Distribution"/>
		<cc:requires rdf:resource="http://web.resource.org/cc/Notice"/>
		<cc:requires rdf:resource="http://web.resource.org/cc/Attribution"/>
		<cc:permits rdf:resource="http://web.resource.org/cc/DerivativeWorks"/>
	</cc:License>
	<rdfs:Class rdf:about="http://purl.org/vocab/lifecycle/schema#Lifecycle">
		<rdfs:label xml:lang="en">Lifecycle</rdfs:label>
		<rdfs:comment xml:lang="en">A lifecycle is a series of states connected by allowable transitions. It may be used to describe the lifecycle of business objects or equally the lifecycle of a butterfly.</rdfs:comment>
		<rdfs:isDefinedBy rdf:resource="http://purl.org/vocab/lifecycle/schema#"/>
		<dct:issued>2008-06-03</dct:issued>
	</rdfs:Class>
	<rdfs:Class rdf:about="http://purl.org/vocab/lifecycle/schema#State">
		<rdfs:label xml:lang="en">State</rdfs:label>
		<rdfs:comment xml:lang="en">A state describes one possible state that a resource can be in at a given time. Resources may be in one state in a given lifecycle at any given time, states are considered mutually exclusive within a lifecycle.</rdfs:comment>
		<rdfs:isDefinedBy rdf:resource="http://purl.org/vocab/lifecycle/schema#"/>
		<dct:issued>2008-06-03</dct:issued>
	</rdfs:Class>
	<rdfs:Class rdf:about="http://purl.org/vocab/lifecycle/schema#Transition">
		<rdfs:label xml:lang="en">Transition</rdfs:label>
		<rdfs:comment xml:lang="en">A transition describes the way in which a resource moves from one state to another state and may also describe the tasks required to make that transition.</rdfs:comment>
		<rdfs:isDefinedBy rdf:resource="http://purl.org/vocab/lifecycle/schema#"/>
		<dct:issued>2008-06-03</dct:issued>
	</rdfs:Class>
	<rdfs:Class rdf:about="http://purl.org/vocab/lifecycle/schema#TaskGroup">
		<rdfs:label xml:lang="en">Task Group</rdfs:label>
		<rdfs:comment xml:lang="en">Represents a collection of tasks grouped together for convenience</rdfs:comment>
		<rdfs:isDefinedBy rdf:resource="http://purl.org/vocab/lifecycle/schema#"/>
		<dct:issued>2008-06-03</dct:issued>
	</rdfs:Class>
	<rdfs:Class rdf:about="http://purl.org/vocab/lifecycle/schema#Task">
		<rdfs:label xml:lang="en">Task</rdfs:label>
		<rdfs:comment xml:lang="en">Represents a task in a workflow</rdfs:comment>
		<rdfs:isDefinedBy rdf:resource="http://purl.org/vocab/lifecycle/schema#"/>
		<dct:issued>2008-06-03</dct:issued>
	</rdfs:Class>
	<rdfs:Class rdf:about="http://purl.org/vocab/lifecycle/schema#Action">
		<rdfs:label xml:lang="en">Action</rdfs:label>
		<rdfs:comment xml:lang="en">Represents an instance of a task taking place against a given resource</rdfs:comment>
		<rdfs:isDefinedBy rdf:resource="http://purl.org/vocab/lifecycle/schema#"/>
		<dct:issued>2008-06-03</dct:issued>
	</rdfs:Class>
	<rdf:Property rdf:about="http://purl.org/vocab/lifecycle/schema#state">
		<rdfs:label xml:lang="en">state</rdfs:label>
		<rdfs:comment>The state property relates any resource with the state that it is currently in.</rdfs:comment>
		<rdfs:domain rdf:resource="http://www.w3.org/1999/02/22-rdf-syntax-ns#Resource"/>
		<rdfs:range rdf:resource="http://purl.org/vocab/lifecycle/schema#State"/>
		<dct:issued>2008-06-03</dct:issued>
		<rdfs:isDefinedBy rdf:resource="http://purl.org/vocab/lifecycle/schema#"/>
	</rdf:Property>
	<rdf:Property rdf:about="http://purl.org/vocab/lifecycle/schema#stateOf">
		<rdfs:label xml:lang="en">state of</rdfs:label>
		<rdfs:comment>The 'state of' property is the inverse of the state property, relating a state to all of the resources currently in that state.</rdfs:comment>
		<rdfs:domain rdf:resource="http://purl.org/vocab/lifecycle/schema#State"/>
		<rdfs:range rdf:resource="http://www.w3.org/1999/02/22-rdf-syntax-ns#Resource"/>
		<owl:inverseOf rdf:resource="http://purl.org/vocab/lifecycle/schema#state"/>
		<dct:issued>2008-06-03</dct:issued>
		<rdfs:isDefinedBy rdf:resource="http://purl.org/vocab/lifecycle/schema#"/>
	</rdf:Property>
	<rdf:Property rdf:about="http://purl.org/vocab/lifecycle/schema#possibleState">
		<rdfs:label xml:lang="en">possible state</rdfs:label>
		<rdfs:comment>The possible state property is used to identify the states that occur within a given lifecycle and are thus the possible states of a resource going through that lifecycle.</rdfs:comment>
		<rdfs:domain rdf:resource="http://purl.org/vocab/lifecycle/schema#Lifecycle"/>
		<rdfs:range rdf:resource="http://purl.org/vocab/lifecycle/schema#State"/>
		<dct:issued>2008-06-03</dct:issued>
		<rdfs:isDefinedBy rdf:resource="http://purl.org/vocab/lifecycle/schema#"/>
	</rdf:Property>
	<rdf:Property rdf:about="http://purl.org/vocab/lifecycle/schema#resultingState">
		<rdfs:label xml:lang="en">resulting state</rdfs:label>
		<rdfs:comment>Once a transition is completed the state of the resource should change to the state specified as the resulting state.</rdfs:comment>
		<rdfs:domain rdf:resource="http://purl.org/vocab/lifecycle/schema#Transition"/>
		<rdfs:range rdf:resource="http://purl.org/vocab/lifecycle/schema#State"/>
		<dct:issued>2008-06-03</dct:issued>
		<rdfs:isDefinedBy rdf:resource="http://purl.org/vocab/lifecycle/schema#"/>
	</rdf:Property>
	<rdf:Property rdf:about="http://purl.org/vocab/lifecycle/schema#possibleTransition">
		<rdfs:label xml:lang="en">possible transition</rdfs:label>
		<rdfs:comment>When in a state there may be many possible transitions.</rdfs:comment>
		<rdfs:domain rdf:resource="http://purl.org/vocab/lifecycle/schema#State"/>
		<rdfs:range rdf:resource="http://purl.org/vocab/lifecycle/schema#Transition"/>
		<dct:issued>2008-06-03</dct:issued>
		<rdfs:isDefinedBy rdf:resource="http://purl.org/vocab/lifecycle/schema#"/>
	</rdf:Property>
	<rdf:Property rdf:about="http://purl.org/vocab/lifecycle/schema#completed">
		<rdfs:label xml:lang="en">completed</rdfs:label>
		<rdfs:comment>This uses a boolean to represent if an action has been completed. This is a simple alternative to the taskProgress property.</rdfs:comment>
		<rdfs:domain rdf:resource="http://purl.org/vocab/lifecycle/schema#Action"/>
		<rdfs:range rdf:resource="http://www.w3.org/2001/XMLSchema#boolean"/>
		<dct:issued>2008-06-03</dct:issued>
		<rdfs:isDefinedBy rdf:resource="http://purl.org/vocab/lifecycle/schema#"/>
	</rdf:Property>
	<rdf:Property rdf:about="http://purl.org/vocab/lifecycle/schema#mandatory">
		<rdfs:label xml:lang="en">mandatory</rdfs:label>
		<rdfs:comment>Sepcifies if a task is mandatory or optional.</rdfs:comment>
		<rdfs:domain rdf:resource="http://purl.org/vocab/lifecycle/schema#Task"/>
		<rdfs:range rdf:resource="http://www.w3.org/2001/XMLSchema#boolean"/>
		<dct:issued>2008-06-03</dct:issued>
		<rdfs:isDefinedBy rdf:resource="http://purl.org/vocab/lifecycle/schema#"/>
	</rdf:Property>
	<rdf:Property rdf:about="http://purl.org/vocab/lifecycle/schema#next">
		<rdfs:label xml:lang="en">next</rdfs:label>
		<rdfs:comment>provides a simple ordering relationship to allow tasks to be ordered in user interfaces.</rdfs:comment>
		<rdfs:domain>
			<owl:Class>
				<owl:unionOf rdf:parseType="Collection">
					<owl:Class rdf:about="http://purl.org/vocab/lifecycle/schema#Task"/>
					<owl:Class rdf:about="http://purl.org/vocab/lifecycle/schema#TaskGroup"/>
				</owl:unionOf>
			</owl:Class>
		</rdfs:domain>
		<rdfs:range>
			<owl:Class>
				<owl:unionOf rdf:parseType="Collection">
					<owl:Class rdf:about="http://purl.org/vocab/lifecycle/schema#Task"/>
					<owl:Class rdf:about="http://purl.org/vocab/lifecycle/schema#TaskGroup"/>
				</owl:unionOf>
			</owl:Class>
		</rdfs:range>
		<dct:issued>2008-06-03</dct:issued>
		<rdfs:isDefinedBy rdf:resource="http://purl.org/vocab/lifecycle/schema#"/>
	</rdf:Property>
	<rdf:Property rdf:about="http://purl.org/vocab/lifecycle/schema#taskGroup">
		<rdfs:label xml:lang="en">task group</rdfs:label>
		<rdfs:comment>A task group related to this transition.</rdfs:comment>
		<rdfs:domain rdf:resource="http://purl.org/vocab/lifecycle/schema#Transition"/>
		<rdfs:range rdf:resource="http://purl.org/vocab/lifecycle/schema#TaskGroup"/>
		<dct:issued>2008-06-03</dct:issued>
		<rdfs:isDefinedBy rdf:resource="http://purl.org/vocab/lifecycle/schema#"/>
	</rdf:Property>
	<rdf:Property rdf:about="http://purl.org/vocab/lifecycle/schema#task">
		<rdfs:label xml:lang="en">task</rdfs:label>
		<rdfs:comment>A task related to this transition.</rdfs:comment>
		<rdfs:domain>
			<owl:Class>
				<owl:unionOf rdf:parseType="Collection">
					<owl:Class rdf:about="http://purl.org/vocab/lifecycle/schema#TaskGroup"/>
					<owl:Class rdf:about="http://purl.org/vocab/lifecycle/schema#Transition"/>
				</owl:unionOf>
			</owl:Class>
		</rdfs:domain>
		<rdfs:range rdf:resource="http://purl.org/vocab/lifecycle/schema#Task"/>
		<dct:issued>2008-06-03</dct:issued>
		<rdfs:isDefinedBy rdf:resource="http://purl.org/vocab/lifecycle/schema#"/>
	</rdf:Property>
	<rdf:Property rdf:about="http://purl.org/vocab/lifecycle/schema#taskProgress">
		<rdfs:label xml:lang="en">task progress</rdfs:label>
		<rdfs:comment>The current progress on this task. Some resources are defined in this ontology for this, but you are free to define your own.</rdfs:comment>
		<rdfs:domain rdf:resource="http://purl.org/vocab/lifecycle/schema#Action"/>
		<rdfs:range rdf:resource="http://purl.org/vocab/lifecycle/schema#TaskProgress"/>
		<dct:issued>2008-06-03</dct:issued>
		<rdfs:isDefinedBy rdf:resource="http://purl.org/vocab/lifecycle/schema#"/>
	</rdf:Property>
	<rdf:Property rdf:about="http://purl.org/vocab/lifecycle/schema#resource">
		<rdfs:label xml:lang="en">resource</rdfs:label>
		<rdfs:comment>The resource on which the action being taken. This is a resource that is being processed through a lifecycle.</rdfs:comment>
		<rdfs:domain rdf:resource="http://purl.org/vocab/lifecycle/schema#Action"/>
		<rdfs:range rdf:resource="http://www.w3.org/1999/02/22-rdf-syntax-ns#Resource"/>
		<dct:issued>2008-06-03</dct:issued>
		<rdfs:isDefinedBy rdf:resource="http://purl.org/vocab/lifecycle/schema#"/>
	</rdf:Property>
	<rdfs:Description rdf:about="http://purl.org/vocab/lifecycle/schema#Completed">
		<rdfs:label xml:lang="en">Completed</rdfs:label>
		<rdfs:comment xml:lang="en">Represents that an individual task has been completed.</rdfs:comment>
		<rdfs:isDefinedBy rdf:resource="http://purl.org/vocab/lifecycle/schema#"/>
		<rdf:type rdf:resource="http://purl.org/vocab/lifecycle/schema#TaskProgress"/>
	</rdfs:Description>
	<rdfs:Description rdf:about="http://purl.org/vocab/lifecycle/schema#Started">
		<rdfs:label xml:lang="en">Started</rdfs:label>
		<rdfs:comment xml:lang="en">Represents that an individual task has been started.</rdfs:comment>
		<rdfs:isDefinedBy rdf:resource="http://purl.org/vocab/lifecycle/schema#"/>
		<rdf:type rdf:resource="http://purl.org/vocab/lifecycle/schema#TaskProgress"/>
	</rdfs:Description>
	<rdfs:Description rdf:about="http://purl.org/vocab/lifecycle/schema#OnHold">
		<rdfs:label xml:lang="en">On Hold</rdfs:label>
		<rdfs:comment xml:lang="en">Represents that an individual task has been placed on hold.</rdfs:comment>
		<rdfs:isDefinedBy rdf:resource="http://purl.org/vocab/lifecycle/schema#"/>
		<rdf:type rdf:resource="http://purl.org/vocab/lifecycle/schema#TaskProgress"/>
	</rdfs:Description>
</rdf:RDF>
