@prefix daq: 	<http://purl.org/eis/vocab/daq#>.
@prefix dc: 							<http://purl.org/dc/elements/1.1/> .
@prefix dct:     					<http://purl.org/dc/terms/>.
@prefix foaf:    					<http://xmlns.com/foaf/0.1/>.
@prefix owl: 	<http://www.w3.org/2002/07/owl#>.
@prefix qpro: <http://purl.org/eis/vocab/qpro#>.
@prefix rdf: 	<http://www.w3.org/1999/02/22-rdf-syntax-ns#>.
@prefix rdfg: <http://www.w3.org/2004/03/trix/rdfg-1>.
@prefix rdfs: <http://www.w3.org/2000/01/rdf-schema#>.
@prefix vann: <http://purl.org/vocab/vann/> .
@prefix voaf: <http://purl.org/vocommons/voaf#>.
@prefix xsd: 	<http://www.w3.org/2001/XMLSchema#>.

qpro:
	a owl:Ontology , voaf:Vocabulary ;
  dct:title """Quality Problem Report (QPRO)"""@en ;
  dc:description """The Quality Problem Report (QPRO) enables the fine-grained description of quality problems found while assessing a dataset."""@en ;
  dct:creator [
    foaf:name "Jeremy Debattista";
    foaf:mbox <mailto:debattij@scss.tcd.ie>
  ] ;
  dct:modified "2017-08-03"^^xsd:date ;
  dct:language "en"^^xsd:language ;
  vann:preferredNamespaceUri "http://purl.org/eis/vocab/qpro#";
  vann:preferredNamespacePrefix "qpro" ;
  foaf:homepage <http://purl.org/eis/vocab/qpro#> .

# Classes
qpro:QualityReport a rdfs:Class ;
	rdfs:comment """Represents a report on the problems detected during the assessment of quality on a dataset."""@en ;
	rdfs:label "Quality Report"@en .

qpro:QualityProblem a rdfs:Class ;
	rdfs:comment """Represents a quality problem detected during the assessment of quality metrics on triples."""@en ;
	rdfs:label "Quality Problem"@en .

qpro:Exception a rdfs:Class ;
		rdfs:comment """Represents an Exception that causes the dataset to have Quality Problems. This is an abstract class"""@en ;
		rdfs:label "Exception (Abstract)"@en .


# Properties
qpro:computedOn a rdf:Property ;
	rdfs:domain qpro:QualityReport ;
	rdfs:range rdfs:Resource ;
	rdfs:comment """Represents the dataset URI on which quality metrics where computed"""@en ;
	rdfs:label "computed on"@en .
	

qpro:hasProblem a rdf:Property ;
	rdfs:domain qpro:QualityReport ;
	rdfs:range qpro:QualityProblem ;
	rdfs:comment """Identifies problem instances in the report"""@en;
	rdfs:label "has problem"@en .


qpro:generatedBy a rdf:Property ;
	rdfs:domain qpro:QualityReport ;
	rdfs:range daq:Observation ;
	rdfs:comment """Links a quality problem to a particular observation in the metadata"""@en;
	rdfs:label "generated by"@en .


qpro:isDescribedBy a rdf:Property;
	rdfs:domain qpro:QualityProblem;
	rdfs:range daq:Metric;
	rdfs:comment """Represent the URI of the metric which instantiated this problem"""@en;
	rdfs:label "is described by"@en .

qpro:problematicThing a rdf:Property;
	rdfs:domain qpro:QualityProblem;
	rdfs:range rdfs:Resource;
	rdfs:comment """Represent the actual problematic instance from the dataset. This could be a list of resources (rdf:Seq), a list of reified statements, or a model representing a list of statements."""@en;
	rdfs:label "Problematic Thing"@en.

qpro:inGraph a rdf:Property;
	rdfs:domain rdf:Statement ;
	rdfs:range rdfg:Graph ;
	rdfs:comment """This property enables the reification of quads by creating a new property to define the context of a triple statement."""@en;
	rdfs:label "in graph"@en.

qpro:exceptionDescription
		a	rdf:Property;
		rdfs:comment """Describes a particular exception raised by the Resource or Triple in question, causing a quality problem"""@en ;
		rdfs:label "Exception Description"@en ;
		rdfs:domain rdfs:Resource ;
		rdfs:range qpro:Exception ;
		rdfs:range xsd:Literal .

qpro:extraExceptionProperty
		a	rdf:Property ;
		rdfs:comment """Enables the description of extra exception properties. This is an abstract property."""@en ;
		rdfs:label "Extra Exception Property (Abstract)"@en .
